Mrk discovery keyring example (#451)

aws-encryption-sdk-net-formally-verified/Source/API/Generated/Crypto/IAwsCryptographicMaterialProviders.cs
@@ -14,6 +14,10 @@ namespace Aws.Crypto
         Aws.Crypto.IKeyring CreateStrictAwsKmsKeyring(Aws.Crypto.CreateStrictAwsKmsKeyringInput input);
         Aws.Crypto.IKeyring CreateAwsKmsDiscoveryKeyring(Aws.Crypto.CreateAwsKmsDiscoveryKeyringInput input);
         Aws.Crypto.IKeyring CreateMrkAwareStrictAwsKmsKeyring(Aws.Crypto.CreateMrkAwareStrictAwsKmsKeyringInput input);
+
+        Aws.Crypto.IKeyring CreateMrkAwareDiscoveryAwsKmsKeyring(
+            Aws.Crypto.CreateMrkAwareDiscoveryAwsKmsKeyringInput input);
+
         Aws.Crypto.IKeyring CreateMultiKeyring(Aws.Crypto.CreateMultiKeyringInput input);
         Aws.Crypto.IKeyring CreateRawAesKeyring(Aws.Crypto.CreateRawAesKeyringInput input);
 
